Let $\alpha, \beta \in k$. We have
\begin{align*}
	\ad(\alpha x + \beta y)(x) &= [\alpha x + \beta y, x] = -\beta y,\\
	\ad(\alpha x + \beta y)(y) &= [\alpha x + \beta y, y] = \alpha y.\\
\end{align*}
On the other hand, let $D\colon L\to L$ be any derivation.
We have $\lambda_1, \lambda_2, \mu_1, \mu_2 \in k$ such that
\[ D(x) = \lambda_1 x + \lambda_2 y,\quad D(y) = \mu_1 x + \mu_2 y. \]
We calculate
\begin{align*}
	\mu_1 x + \mu_2 y &= D(y) = D([x, y]) = [D(x), y] + [x, D(y)]\\
	&= [\lambda_1 x + \lambda_2 y, y] + [x, \mu_1 x + \mu_2 y] = \lambda_1 y + \mu_2 y.
\end{align*}
Hence $\mu_1 = \lambda_1 = 0$ and $D = \ad(\mu_2 x - \lambda_2 y)$, finishing
the proof.
