If $f\colon M\to N$ is any morphism of $R$-modules, then we have a map
$f_n\colon M/I^nM \to N/I$. These maps fit into a commutative diagram
\[\begin{tikzcd}
	M/M\ar[d] & M/IM\ar[l]\ar[d] & M/I^2N\ar[d]\ar[l] & M/I^3M\ar[l]\ar[d] & \ldots\ar[l]\\
	N/N & N/IN\ar[l] & N/I^2N\ar[l] & N/I^3N\ar[l] & \ldots\ar[l].
\end{tikzcd}\]
By the universal property of the direct limit $\hat{N} $, we get a unique induced morphism
$\hat{f}\colon \hat{M}\to \hat{N}$ such that $\pi_n(\hat{f}(x)) = f_n(\pi_n(x))$.
This gives immediately that $\hat{\cdot}$ is functorial and if $f = 0$, then
$\hat{f} = 0$.

Furthermore, we claim that if $f$ is injective, then $\hat{f}$ is injective. Indeed,
by Artin-Rees, we find $s$ such that for all $n\geq s$ we have
\[ (I^nN)\cap f(M) = I^{n-s}((I^sN)\cap f(M)). \]
Now let $x \in \hat{M}$ such that $\hat{f}(x) = 0$. First, let $n \in \mathbb{N}_0$.
If $\pi_{n + s}(x) = m + I^{n + s}M$, then $0 = \pi_{n + s}(\hat{f}(x)) = f_{n + s}(\pi_{n + s}(x)) = f(m) + I^{n + s}M$.
Hence,
\[ f(m) \in (I^{n + s}N) \cap f(M) = I^n((I^sN)\cap f(M)), \]
i.e., we find $i_k \in I^n$, $m'_k \in M$ such that $f(m) = \sum_k i_kf(m'_k) = f(i_km'_k)$. But
$f$ is injective, hence we conclude $m = \sum_k i_k m'_k$. The fact that $\hat{M}$ is an inverse
limit (so the projections form a cone over the inverse system) tells us that
$\pi_n(x) = m + I^nM = \sum_k i_k m'_k + I^nM = 0$. Doing this for all $n$, we find that
$x = 0$ as required.

Hence, we get our induced morphisms $\hat{\iota}$ and $\hat{\varphi}$ and we have
already shown that $\hat{\iota}$ is injective and that $\im\hat{\iota} \subseteq \ker\hat{\varphi}$.

In what follows, let $s$ be the maximum of the Artin-Rees constants of the
submodules $\iota(M_1) \subseteq M$ and $\varphi(M) \subseteq M_2$.

Next, we will show that $\ker\hat{\varphi} \subseteq \im\hat{\iota}$. Indeed,
ket $x \in \hat{M'}$ such that $\hat{\varphi}(x) = 0$. Write
$\pi_n(x) = x_n + I^nM$, then we have $\varphi(x_n) \in I^nM_2$.

Let $n \in \mathbb{N}$. Then using Artin-Rees we have
$\varphi(x_{n+s}) \in I^n(I^sM_2\cap \varphi(M))$, so we find
$x_{n+s,k}' \in M_2$ and $i_{n+s,k} \in I^n$ such that
$\varphi(x_{n+s}) = \sum_k i_{n+s,k}\varphi(x_{n+s,k}')$. Then
$x_{n+s} - \sum_k i_{n+s,k}x_{n+s,k}' \in \ker\varphi$, so we find $y_{n+s} \in M_1$ such
that $\iota(y_{n+s}) = x_{n+s} - \sum_k i_{n+s,k}x_{n+s,k}'$. But then
\[ \iota_n(y_{n+s} + I^nM_1) = x_{n+s} - \sum_k i_{n+s,k}x_{n+s,k}' + I^nM = x_{n+s} + I^nM = x_n + I^nM. \]
Hence, we are done as long as we can show that $(y_{n+s} + I^nM_1)_{n \in \mathbb{N}}$
assemble into an element of $\hat{M_1}$, i.e., that for $n\leq m$ we have
$y_{m+s} + I^nM_1 = y_{n+s} + I^nM_1$. Indeed, we have
\[ \iota(y_{m+s} - y_{n+s}) = x_{m+s} - i_{m+s}x_{m+s}' - x_{n+s} + i_{n+s}x_{n+s}' \in I^{n+s}M, \]
so Artin-Rees tells us that we find $i_{n, m, k} \in I^nM$ and $y_{n, m, k} \in M_1$ such
that $\iota(y_{m+s} - y_{n+s}) = \iota(\sum_k i_{n, m,k}y_{n, m,k})$. But $\iota$ is injective,
so $y_{m+s} - y_{n+s} \in I^nM$ as required, completing the proof that
$\ker\hat{\varphi} \subseteq \im\hat{\iota}$.

It remains to show that $\hat{\varphi}$ is surjective.
Indeed, let $z = (z_n + I^nM_2) \in \hat{M_2}$. We will construct a preimage
$y = (y_n + I^nM) \in \hat{M}$ by induction. In fact, we will do something slightly
stronger: we will construct a sequence $(y_n)$ of elements of $M$ such that
$y_{n+1} + I^nM = y_n + I^nM$ and $\varphi(y_n) = z_n$ for every $n$.

We set $y_0$ to be a preimage of $z_0$ under $\varphi$. Now let $n > 0$
and suppose that we have already defined $y_n \in M$ such that
$\varphi(y_n) = z_n$. We need to find $y_{n+1} \in M$ such
that $\varphi(y_{n+1}) = z_{n+1}$ and $y_n + I^nM = y_{n+1} + I^nM$.

We have $z_n + I^nM = z_{n+1} + I^nM$, so $z_{n+1} - z_n \in I^nM$, i.e.,
$z_{n + 1} - z_n = \sum r_iw_i$ for $r_i \in I^n$, $w_i \in M_2$. By surjectivity
of $\varphi$, we find $t_i \in M$ such that $s\coloneqq \sum r_it_i \in I^nM$ satisfies
$\varphi(s) = z_{n + 1} - z_n$. Define $y_{n+1}\coloneqq y_n + s$. Then $y_{n+1} + I^nM = y_n + I^nM$
since $s \in I^nM$,
and $\varphi(y_{n+1}) = \varphi(y_n) + \varphi(s) = z_n + z_{n+1} - z_n = z_{n+1}$.
