We have $\scp{h_\alpha, h_\alpha}_{\ad} = \alpha(h_\alpha) \neq 0$ by 4.15(b).

\[ 2 \frac{\scp{h_\beta, h_\alpha}_{\ad}}{\scp{h_\alpha, h_\alpha}_{\ad}}
= 2\frac{\beta(h_\alpha)}{\alpha(h_\alpha)} = \frac{2(q-p)}{2} \in \mathbb{Z}, \]
where the $\alpha$-string through $\beta$ is
\[ \beta-q\alpha, \ldots, \beta, \ldots, \beta+p\alpha. \]
This shows (a).

For (b), let $x, y \in H$, we have
\[ \scp{x, y}_{\ad} = \sum_{\beta \in \Phi} \beta(x)\beta(y) \]
by 4.13(a) and 4.16(a).
Hence,
\[ \scp{h_\alpha, h_\alpha}_{\ad} = \sum_{\beta \in \Phi} \beta(h_\alpha)^2 = \sum_{\beta \in \Phi}\scp{h_\beta, h_\alpha}_{\ad}^2. \]
Pulling out the denominator from the left hand side of the claim and substituting
yields (b).

Part (c) follows immediately from (a) and (b).

For (d), notice that
\[ \beta - 2\frac{\scp{h_\beta, h_\alpha}}{\scp{h_\alpha, h_\alpha}}\alpha = \beta + (p-q)\alpha \]
is in the $\alpha$-string through $\beta$, so we are done.

