\begin{enumerate}[label=(\arabic*)]
	\item The adjoint representation $\ad_{\mathfrak{L}}\colon \mathfrak{L}\to\End \mathfrak{L}$
		is given by $x\mapsto (y\mapsto [x, y])$.

		It is indeed a homomorphism: if $x, y, z \in \mathfrak{L}$, then we may
		calculate
		\begin{align*}
			\ad_{\mathfrak{L}}([x, y])(z)
			&= [[x, y], z]\\
			&= -[z, [x, y]]\\
			&= [x, [y, z]] + [y, [z, x]]\\
			&= \ad_{\mathfrak{L}}(x)(\ad_{\mathfrak{L}}(y)(z)) - \ad_{\mathfrak{L}}(y)(\ad_{\mathfrak{L}}(x)(z))\\
			&= (\ad_{\mathfrak{L}}(x)\circ\ad_{\mathfrak{L}}(y) - \ad_{\mathfrak{L}}(y) \circ \ad_{\mathfrak{L}}(x))(z)\\
			&= [\ad_{\mathfrak{L}}(x), \ad_{\mathfrak{L}}(y)](z),
		\end{align*}
		where we have used the Jacobi identity.
\end{enumerate}
