If $M$ is noetherian, then in particular all submodules of $N$ are finitely generated.
Furthermore, all submodules of $M/N$ are of the form $Q/N$, where $Q$ is submodule of
$M$ containing $N$. $Q$ is finitely generated, say by $x_1, \ldots, x_r$. Then
$Q/N$ is generated by $x_1 + N, \ldots, x_r + N$.

Conversely, if both $N$ and $M/N$ are noetherian, and $L_1 \subseteq L_2 \subseteq \ldots$
is an increasing chain of submodules of $M$, define $Q_i \coloneqq L_i + N$ and
$N_i \coloneqq L_i\cap N$. Then $Q_i/N$ and $N_i$ are chains of submodules of
$M/N$ and $N$, respectively, so they terminate and we find $r$ such that
$\forall i\geq r\colon Q_i/N = Q_r/N$ and $s$ such that $\forall i\geq s\colon N_i = N_s$.
Define $k\coloneqq \max\set{r, s}$.

We will show that $\forall i\geq k\colon L_i = L_k$. Indeed, let $\ell \in L_i$.
Then $\ell + N \in Q_i/N = Q_k/N = (L_k + N)/N$, so there are $\tilde{\ell} \in N, \ell' \in L_k, \hat{\ell} \in N$
such that $\ell - \tilde{\ell} = \ell' + \hat{\ell}$. Rearranging, we find that
$\ell - \ell' = \tilde{\ell} + \hat{\ell} \in N$, and since $L_k \subseteq L_i$ we
conclude that $\ell - \ell' \in N \cap L_i = N \cap L_k$. Therefore,
$\ell = (\ell - \ell') + \ell' \in L_k$ and we are done.
