As always, all rings $R$ are commutative with unity.

Let $S$ be a multiplicatively closed subset of $R$ (i.e.,  $S$ is closed under
multiplication and $1 \in S$). We define a relation $\equiv$ on $R\times S$ by saying
that $(r_1, s_1)\equiv (r_2, s_2)\iff \exists x \in S\colon (r_1s_2 - r_2s_1)x = 0$.
Reflexivity and symmetry are immediate, for transitivity, assume that
\[ (r_1s_2 - r_2s_1)x = 0 = (r_2s_3-r_3s_2)y. \]
Multiplying the left hand side with $s_3y$ and the right hand side with $s_1x$
and the subtracting the two yields the desired identity
\[ (r_1s_3 - r_3s_1)s_2xy = 0, \]
since $s_2xy \in S$.

This shows that $\equiv$ is an equivalence relation, and we will denote equivalence
classes of $(r_1, s_1)$ by $\frac{r_1}{s_2}$ and the quotient by
$S^{-1}R$. We make  $S^{-1}R$ into a ring by setting
\begin{align*}
	\frac{r_1}{s_1}+\frac{r_2}{s_2}&\coloneqq \frac{r_1s_2+r_2s_1}{s_1s_2},\\
	\frac{r_1}{s_1}\cdot\frac{r_2}{s_2}&\coloneqq \frac{r_1r_2}{s_1s_2}.
\end{align*}
Furthermore, we have a ring homohmorphism $R\to S^{-1}R$ given by $r\mapsto\frac{r}{1}$.
