First of all, let $x, y, z \in L$. Then we have
\begin{align*}
	\ad(x)([y, z]) &= [x, [y, z]]\\
	&= -[z, [x, y]] - [y, [z, x]]\\
	&= [[x, y], z] + [y, [x, z]]\\
	&= [\ad(x)(y), z] + [y, \ad(x)(z)],
\end{align*}
so $\ad(x)$ is a derivation and we conclude that $\ad(L) \subseteq \Der L$. Since
adjoints are obviously closed under addition and scalar multiplication,
$\ad(L)$ is a subspace of $\Der L$.

Furthermore, let $D \in \Der L$ and $x, y \in L$. Then we have
\begin{align*}
	[D, \ad_{L}(x)](y) &= (D \circ \ad_{L}(x) - \ad_{L}(x) \circ D)(y)\\
	&= D([x, y]) - [x, D(y)]\\
	&= [D(x), y] + [x, D(y)] - [x, D(y)]\\
	&= [D(x), y]\\
	&= \ad_{L}(D(x))(y),
\end{align*}
so we conclude that $[D, \ad(x)] = \ad(D(x))$, hence $\ad(L)$ is a Lie ideal
of $\Der L$.
