Let $e_\alpha \in L_\alpha$, $e_{-\alpha} \in L_{-\alpha}$ and $h_\alpha \in H$
be the elements from Lemma 4.18. It follows immediately from 4.18 that all of these
elements are nonzero, so since $\dim L_{\pm\alpha} = 1$, these elements form a basis of
the subalgebra generated by $L_\alpha$ and $L_{-\alpha}$, which we will call
$L$.

We have $[h_\alpha, e_\alpha] \in L_\alpha$ by 4.13(b), so $[h_\alpha, e_\alpha] = \lambda e_\alpha$
for some $\lambda \in \mathbb{C}$. We may calculate
\[ \lambda = \lambda\scp{e_\alpha, e_{-\alpha}}_{\ad} = \scp{[h_\alpha, e_\alpha], e_{-\alpha}}_{\ad} = \scp{h_\alpha, [e_\alpha, e_{-\alpha}]}_{\ad} = \scp{h_\alpha, h_\alpha}= \alpha(h_\alpha)\neq 0, \]
using 4.18(c), 4.18(a) and 4.15(b). By a similar argument,
$[h_\alpha, e_{-\alpha}] = -\alpha(h_\alpha)$. Now define a linear map
$\Phi\colon \mathfrak{sl}_2\to L$ via
\[ e\mapsto \sqrt{\frac{2}{\alpha(h_\alpha)}}e_\alpha,\qquad f\mapsto \sqrt{\frac{2}{\alpha(h_\alpha)}}e_{-\alpha},\qquad h\mapsto \frac{2}{\alpha(h_\alpha)}h_\alpha. \]
This is clearly an isomorphism of vector spaces, and it is an isomorphism of Lie algebras,
since
\begin{align*}
	[\Phi(e), \Phi(f)] &= \frac{2}{\alpha(h_\alpha)}[e_\alpha, e_{-\alpha}] = \Phi(h) = \Phi([e, f]),\\
	[\Phi(h), \Phi(e)] &= \left(\frac{2}{\alpha(h_\alpha)}\right)^{3/2}[h_\alpha, e_\alpha] = 2\sqrt{\frac{2}{\alpha(h_\alpha)}}e_\alpha = 2\Phi(e) = \Phi([h, e]),\\
	[\Phi(h), \Phi(f)] &= \left(\frac{2}{\alpha(h_\alpha)}\right)^{3/2}[h_\alpha, e_{-\alpha}] = -2\sqrt{\frac{2}{\alpha(h_\alpha)}}e_{-\alpha} = -2\Phi(f) = \Phi([h, f]),
\end{align*}
completing the proof.
